Add derivations to Model.QUIC

src/Model.PNE.fst
@@ -70,10 +70,14 @@ let create j u =
   else
     (u, random (Spec.key_length u.calg)) <: unsafe_state j
 
-let coerce j u ts =
-  (u, Model.Helpers.hide #(key_len u) (
-    QUIC.Spec.derive_secret u.halg ts
-        QUIC.Spec.label_hp (key_len u)) <: unsafe_state j)
+let coerce j u k =
+  (u, k) <: unsafe_state j
+
+let quic_coerce j u ts =
+  let k = Model.Helpers.hide #(key_len u)
+    (QUIC.Spec.derive_secret u.halg ts
+        QUIC.Spec.label_hp (key_len u)) in
+  coerce j u k
 
 let random_bits (): bits =
   LowParse.BitFields.get_bitfield #8 (UInt8.v (Lib.RawIntTypes.u8_to_UInt8 (Seq.index (random 1) 0))) 0 5
